Add simpler definitions.

src/dafny/refinement/evm.dfy
@@ -21,10 +21,10 @@ module EVM {
 
     import opened EVMSeq 
 
-    datatype EVMProg<!S> = 
-            AInst(i: EVMInst)
-        |   Jumpi(cond: S -> bool, tgt: nat)
-        |   Jump(tgt: nat)
+    // datatype EVMProg<!S> = 
+    //         AInst(i: EVMInst)
+    //     |   Jumpi(cond: S -> bool, tgt: nat)
+    //     |   Jump(tgt: nat)
 
     /**
      *  EVM instructions.
@@ -35,26 +35,61 @@ module EVM {
             AInst(i: EVMInst)
         |   Jumpi(cond: S -> bool, tgt: int)    
         |   Jump(tgt: int)
+        // |   Nop()
+
+    /**
+     *  Run one step of a program.
+     *  
+     *
+     *  @note   If the `pc` is outside the set of instructions, stop.
+     */
+    function method stepEVM<S>(pc: nat, p: seq<EVMProg2>, s: S): (int, S)
+    {
+        if pc < 0 || pc >= |p| then  
+            (pc, s)
+        else 
+            match p[pc] 
+                case AInst(i)       =>  (pc + 1, runInst(i, s))
+                case Jumpi(c, tgt)  =>  if !c(s) then (pc + 1, s) 
+                                        else (pc + tgt, s)
+                case Jump(tgt)      =>  (pc + tgt, s) 
+                // case Nop()          =>  (pc + 1, s)
+
+    }
+
+    function method stepEVM2<S, T>(pc: int, p: seq<(EVMProg2, T)>, s: S): (int, S)
+    {
+        if pc < 0 || pc >= |p| then  
+            (pc, s)
+        else 
+            match p[pc].0 
+                case AInst(i)       =>  (pc + 1, runInst(i, s))
+                case Jumpi(c, tgt)  =>  if !c(s) then (pc + 1, s) 
+                                        else (pc + tgt, s)
+                case Jump(tgt)      =>  (pc + tgt, s) 
+                // case Nop()          =>  (pc + 1, s)
+
+    }
 
     /**
      *  Semantics of EVM programs.
      */
-    function method runEVM<S>(pc: nat, p: map<nat, EVMProg>, s: S, n: nat): (S, nat)
-        decreases n 
-    {
-        if pc == 0 || n == 0 || pc !in p then (s, 0)
-            //  We could have different types of termination
-        else 
-            //  Execute instruction at PC and increment PC accordingly
-            match p[pc] 
-                case AInst(i) => 
-                    runEVM(pc + 1, p, runInst(i, s), n - 1)
-                case Jumpi(c, tgt) => 
-                    if !c(s) then runEVM(pc + 1, p, s, n - 1) 
-                    else runEVM(tgt, p, s, n - 1)
-                case Jump(tgt) => 
-                    runEVM(tgt, p, s, n - 1) 
-    }
+    // function method runEVM<S>(pc: nat, p: map<nat, EVMProg>, s: S, n: nat): (S, nat)
+    //     decreases n 
+    // {
+    //     if pc == 0 || n == 0 || pc !in p then (s, 0)
+    //         //  We could have different types of termination
+    //     else 
+    //         //  Execute instruction at PC and increment PC accordingly
+    //         match p[pc] 
+    //             case AInst(i) => 
+    //                 runEVM(pc + 1, p, runInst(i, s), n - 1)
+    //             case Jumpi(c, tgt) => 
+    //                 if !c(s) then runEVM(pc + 1, p, s, n - 1) 
+    //                 else runEVM(tgt, p, s, n - 1)
+    //             case Jump(tgt) => 
+    //                 runEVM(tgt, p, s, n - 1) 
+    // }
 
     /**
      *  Compute the state after executing a given number of intructions.
@@ -70,53 +105,36 @@ module EVM {
      *              `pc` to `pc + k`.
      *  
      */
-    function method runEVM2<S>(pc: int, p: seq<EVMProg2>, s: S, n: nat): (S, nat)
-        decreases n 
-    {
-        if n == 0 || pc >= |p| || pc < 0 then (s, |p|)
-            //  We could have different types of termination.
-        else 
-            //  Execute instruction at PC and increment PC accordingly.
-            match p[pc] 
-                case AInst(i)       =>  runEVM2(pc + 1, p, runInst(i, s), n - 1)
-                case Jumpi(c, tgt)  =>  if !c(s) then runEVM2(pc + 1, p, s, n - 1) 
-                                        else runEVM2(pc + tgt, p, s, n - 1)
-                case Jump(tgt)      =>  runEVM2(pc + tgt, p, s, n - 1) 
-    }
+    // function method runEVM2<S>(pc: int, p: seq<EVMProg2>, s: S, n: nat): (S, nat)
+    //     decreases n 
+    // {
+    //     if n == 0 || pc >= |p| || pc < 0 then (s, |p|)
+    //         //  We could have different types of termination.
+    //     else 
+    //         //  Execute instruction at PC and increment PC accordingly.
+    //         match p[pc] 
+    //             case AInst(i)       =>  runEVM2(pc + 1, p, runInst(i, s), n - 1)
+    //             case Jumpi(c, tgt)  =>  if !c(s) then runEVM2(pc + 1, p, s, n - 1) 
+    //                                     else runEVM2(pc + tgt, p, s, n - 1)
+    //             case Jump(tgt)      =>  runEVM2(pc + tgt, p, s, n - 1) 
+    // }
 
     //  returns s', pc', n'
-    function method runEVM3<S>(pc: int, p: seq<EVMProg2>, s: S, n: nat): (S, int, nat)
-        decreases n 
-    {
-        if n == 0 || pc >= |p| || pc < 0 then (s, pc, n)
-            //  We could have different types of termination.
-        else 
-            //  Execute instruction at PC and increment PC accordingly.
-            match p[pc] 
-                case AInst(i)       =>  runEVM3(pc + 1, p, runInst(i, s), n - 1)
-                case Jumpi(c, tgt)  =>  if !c(s) then runEVM3(pc + 1, p, s, n - 1) 
-                                        else runEVM3(pc + tgt, p, s, n - 1)
-                case Jump(tgt)      =>  runEVM3(pc + tgt, p, s, n - 1) 
-    }
+    // function method runEVM3<S>(pc: int, p: seq<EVMProg2>, s: S, n: nat): (S, int, nat)
+    //     decreases n 
+    // {
+    //     if n == 0 || pc >= |p| || pc < 0 then (s, pc, n)
+    //         //  We could have different types of termination.
+    //     else 
+    //         //  Execute instruction at PC and increment PC accordingly.
+    //         match p[pc] 
+    //             case AInst(i)       =>  runEVM3(pc + 1, p, runInst(i, s), n - 1)
+    //             case Jumpi(c, tgt)  =>  if !c(s) then runEVM3(pc + 1, p, s, n - 1) 
+    //                                     else runEVM3(pc + tgt, p, s, n - 1)
+    //             case Jump(tgt)      =>  runEVM3(pc + tgt, p, s, n - 1) 
+    // }
 
-    /**
-     *  Run one step of a program.
-     *  
-     *
-     *  @note   If the `pc` is outside the sdt of instructions, stop.
-     */
-    function method stepEVM<S>(pc: nat, p: seq<EVMProg2>, s: S): (int, S)
-    {
-        if pc < 0 || pc >= |p| then  
-            (pc, s)
-        else 
-            match p[pc] 
-                case AInst(i)       =>  (pc + 1, runInst(i, s))
-                case Jumpi(c, tgt)  =>  if !c(s) then (pc + 1, s) 
-                                        else (pc + tgt, s)
-                case Jump(tgt)      =>  (pc + tgt, s) 
-
-    }
+    
 
     /**
      *  All jumps are close jumps.
@@ -124,10 +142,10 @@ module EVM {
      *  @param  p   A program.
      *  @returns    Whether all instructions in `p` are clode jumps.
      */
-    predicate isClosed(p: seq<EVMProg2>)
-    {
-        forall i :: 0 <= i < |p| ==> closeJump(p, i)
-    }
+    // predicate isClosed(p: seq<EVMProg2>)
+    // {
+    //     forall i :: 0 <= i < |p| ==> closeJump(p, i)
+    // }
 
     /**
      *  Whether an instruction transfers control within a program boundary.
@@ -140,14 +158,14 @@ module EVM {
      *              program's instructions locations and `p` which corresponds to
      *              the program's end point (termination).  
      */
-    predicate closeJump(p: seq<EVMProg2>, i: nat)
-        requires 0 <= i < |p| 
-    {
-        match p[i]
-                case Jumpi(cond, tgt)   => 0 <= i + tgt <= |p| 
-                case Jump(tgt)          => 0 <= i + tgt <= |p| 
-                case _                  => true
-    }
+    // predicate closeJump(p: seq<EVMProg2>, i: nat)
+    //     requires 0 <= i < |p| 
+    // {
+    //     match p[i]
+    //             case Jumpi(cond, tgt)   => 0 <= i + tgt <= |p| 
+    //             case Jump(tgt)          => 0 <= i + tgt <= |p| 
+    //             case _                  => true
+    // }
 
     /**
      *  The execution of n steps of a closed program |p| either termninates with 
@@ -158,90 +176,90 @@ module EVM {
      *  @param  s   An initial state.
      *  @param  n   The maximum number of steps to be executed.
      */
-    lemma pcBoundsOnTermination<S>(pc: nat, p: seq<EVMProg2>, s: S, n: nat) 
-        requires isClosed(p)
-        requires 0 <= pc <= |p|
-        ensures 0 <= runEVM3<S>(pc, p, s, n).1 <= |p|
-        ensures 0 <= runEVM3<S>(pc, p, s, n).1 < |p| ==> runEVM3<S>(pc, p, s, n).2 == 0 
-        ensures runEVM3<S>(pc, p, s, n).1 == |p| ==> runEVM3<S>(pc, p, s, n).2 >= 0  
-        decreases n 
-    {
-        if |p| == pc || n == 0 {
-            //  Thanks Dafny
-        } else {
-            assert pc < |p|; 
-            match p[pc] 
-                case AInst(i)           =>  
-                    pcBoundsOnTermination(pc + 1, p, runInst(i, s), n - 1);
-                case Jumpi(cond, tgt)   =>  
-                    assert closeJump(p, pc);
-                    assert 0 <= pc + tgt <= |p|;
-                    pcBoundsOnTermination(if cond(s) then pc + tgt else pc + 1, p, s, n - 1);
-                case Jump(tgt)          => 
-                    assert closeJump(p, pc);
-                    assert 0 <= pc + tgt <= |p|;
-                    pcBoundsOnTermination(pc + tgt, p, s, n - 1);
-        }
-    }
+    // lemma pcBoundsOnTermination<S>(pc: nat, p: seq<EVMProg2>, s: S, n: nat) 
+    //     requires isClosed(p)
+    //     requires 0 <= pc <= |p|
+    //     ensures 0 <= runEVM3<S>(pc, p, s, n).1 <= |p|
+    //     ensures 0 <= runEVM3<S>(pc, p, s, n).1 < |p| ==> runEVM3<S>(pc, p, s, n).2 == 0 
+    //     ensures runEVM3<S>(pc, p, s, n).1 == |p| ==> runEVM3<S>(pc, p, s, n).2 >= 0  
+    //     decreases n 
+    // {
+    //     if |p| == pc || n == 0 {
+    //         //  Thanks Dafny
+    //     } else {
+    //         assert pc < |p|; 
+    //         match p[pc] 
+    //             case AInst(i)           =>  
+    //                 pcBoundsOnTermination(pc + 1, p, runInst(i, s), n - 1);
+    //             case Jumpi(cond, tgt)   =>  
+    //                 assert closeJump(p, pc);
+    //                 assert 0 <= pc + tgt <= |p|;
+    //                 pcBoundsOnTermination(if cond(s) then pc + tgt else pc + 1, p, s, n - 1);
+    //             case Jump(tgt)          => 
+    //                 assert closeJump(p, pc);
+    //                 assert 0 <= pc + tgt <= |p|;
+    //                 pcBoundsOnTermination(pc + tgt, p, s, n - 1);
+    //     }
+    // }
 
-    lemma localProp<S>(pc: nat, p: seq<EVMProg2>, s: S, k1: nat, k2: nat)
-        requires 0 <= k1 < k2 < |p|
-        requires isClosed(p[k1..k2])
-        requires k1 <= pc < k2
-        ensures k1 <= stepEVM(pc, p, s).0 <= k2 
-        // decreases n
-    {
-        if false {
-            //  Thanks Dafny
-        } else if pc == k2 { 
-            // calc <= {
-            //     runEVM3(pc, p, s, n).1;
-            //     runEVM3(pc, p[k1..k2], s, n).1;
-            //     // { assert isClosed(p[k1..k2]) ;}
-            //     // k2;
-            // }
-        } else {
-            assert k1 <= pc < k2; 
-            match p[pc] 
-                case AInst(i)           =>  
-                    // localProp(pc + 1, p, runInst(i, s), k1, k2);
-                    // assume k1 <= runEVM3(k1, p, s, n).1 <= k2 ;
-                    // pcBoundsOnTermination(pc + 1, p, runInst(i, s), n - 1);
-                case Jumpi(cond, tgt)   =>  
-                    // assert closeJump(p, pc);
-                    assume k1 <= stepEVM(pc, p, s).0 <= k2 ;
-                    // assert 0 <= pc + tgt <= |p|;
-                    // pcBoundsOnTermination(if cond(s) then pc + tgt else pc + 1, p, s, n - 1);
-                case Jump(tgt)          => 
-                    // assume k1 <= stepEVM(pc, p, s).0 <= k2 ;
-                    calc == {
-                        p[pc];
-                        p[k1..k2][pc - k1];
-                    }
-                    calc == {
-                        stepEVM(pc, p, s);
-                        (pc + tgt, s);
-                        calc == {
-                            p[pc];
-                            p[k1..k2][pc - k1];
-                        }
-                        stepEVM(pc - k1, p[k1..k2], s);
-                        // (pc + tgt, s);
-                    }
-                    calc == {
-                        stepEVM(pc - k1, p[k1..k2], s).0;
-                        pc - k1 + tgt;
-                        // calc == {
-                        //     p[pc];
-                        //     p[k1..k2][pc - k1];
-                        // }
+    // lemma localProp<S>(pc: nat, p: seq<EVMProg2>, s: S, k1: nat, k2: nat)
+    //     requires 0 <= k1 < k2 < |p|
+    //     requires isClosed(p[k1..k2])
+    //     requires k1 <= pc < k2
+    //     ensures k1 <= stepEVM(pc, p, s).0 <= k2 
+    //     // decreases n
+    // {
+    //     if false {
+    //         //  Thanks Dafny
+    //     } else if pc == k2 { 
+    //         // calc <= {
+    //         //     runEVM3(pc, p, s, n).1;
+    //         //     runEVM3(pc, p[k1..k2], s, n).1;
+    //         //     // { assert isClosed(p[k1..k2]) ;}
+    //         //     // k2;
+    //         // }
+    //     } else {
+    //         assert k1 <= pc < k2; 
+    //         match p[pc] 
+    //             case AInst(i)           =>  
+    //                 // localProp(pc + 1, p, runInst(i, s), k1, k2);
+    //                 // assume k1 <= runEVM3(k1, p, s, n).1 <= k2 ;
+    //                 // pcBoundsOnTermination(pc + 1, p, runInst(i, s), n - 1);
+    //             case Jumpi(cond, tgt)   =>  
+    //                 // assert closeJump(p, pc);
+    //                 assume k1 <= stepEVM(pc, p, s).0 <= k2 ;
+    //                 // assert 0 <= pc + tgt <= |p|;
+    //                 // pcBoundsOnTermination(if cond(s) then pc + tgt else pc + 1, p, s, n - 1);
+    //             case Jump(tgt)          => 
+    //                 // assume k1 <= stepEVM(pc, p, s).0 <= k2 ;
+    //                 calc == {
+    //                     p[pc];
+    //                     p[k1..k2][pc - k1];
+    //                 }
+    //                 calc == {
+    //                     stepEVM(pc, p, s);
+    //                     (pc + tgt, s);
+    //                     calc == {
+    //                         p[pc];
+    //                         p[k1..k2][pc - k1];
+    //                     }
+    //                     stepEVM(pc - k1, p[k1..k2], s);
+    //                     // (pc + tgt, s);
+    //                 }
+    //                 calc == {
+    //                     stepEVM(pc - k1, p[k1..k2], s).0;
+    //                     pc - k1 + tgt;
+    //                     // calc == {
+    //                     //     p[pc];
+    //                     //     p[k1..k2][pc - k1];
+    //                     // }
 
-                    }
-                    assume k1 <= stepEVM(pc, p, s).0 <= k2 ;
-                    // assert closeJump(p[k1..k2], pc);
-                    // assert 0 <= pc + tgt <= |p|;
-                    // pcBoundsOnTermination(pc + tgt, p, s, n - 1);
-                    // assume k1 <= runEVM3(k1, p, s, n).1 <= k2 ;
-        }   
-    } 
+    //                 }
+    //                 assume k1 <= stepEVM(pc, p, s).0 <= k2 ;
+    //                 // assert closeJump(p[k1..k2], pc);
+    //                 // assert 0 <= pc + tgt <= |p|;
+    //                 // pcBoundsOnTermination(pc + tgt, p, s, n - 1);
+    //                 // assume k1 <= runEVM3(k1, p, s, n).1 <= k2 ;
+    //     }   
+    // } 
 }
