src/dafny/refinement/evmir-refinement-general.dfy
@@ -30,167 +30,204 @@ module EVMIRSimulationFull {
     //  General proofs
     //  For this we need to define a translation from EVM-IR to EVM
 
+    function method continuationClosure(p: seq<(EVMProg2, seq<EVMIRProg>)>, p1:  seq<EVMIRProg>):
+        seq<(EVMProg2, seq<EVMIRProg>)>
+    {
+        if p == [] then 
+            []
+        else 
+            [(p[0].0, p[0].1 + p1)]
+            + continuationClosure(p[1..], p1) 
+    }
+
     /**
-     *  Translate and EVMir program into a EVM program.
+     *  Translate and EVMIR program into a EVM program.
      *
-     *  @param  p   An EVM-IR program.
+     *  @param  p   An EVMIR program.
      *  @returns    Its translation into EVM (while and if are mapped to jumps).
      */
-    function method toEVM<S>(p: EVMIRProg): seq<EVMProg2> 
+    function method toEVM<S>(p: seq<EVMIRProg>): seq<(EVMProg2, seq<EVMIRProg>)> 
     {
-        match p 
-            case Block(i) => [EVMProg2.AInst(i)]
+        if p == [] then 
+            []
+        else 
+            match p[0]
+                case Block(i) => [(EVMProg2.AInst(i), [Block(i)])] + toEVM(p[1..])
 
-            case While(c, xb) => 
-                //   Translate xb into EVM. xbb goes from 0 to |xbb| - 1
-                var xbb := toEVM(xb);
-                //  transaliton of While is 0 -> jumpi, 1..|xbb| xbb, xbb + 1 -> Jump
-                [EVMProg2.Jumpi(negF(c), |xbb| + 2)] +  //  0 
-                    xbb +                               //  1..|xbb|
-                [EVMProg2.Jump(-(|xbb| + 1))]           //  |xbb| + 1
+                case While(c, b) => 
+                    //   Translate b into EVM. xbb goes from 0 to |xbb| - 1
+                    var xbb := toEVM(b);   
+                    //  translation of While is 0 -> jumpi, 1..|xbb| xbb, xbb + 1 -> Jump
+                    [(EVMProg2.Jumpi(negF(c), |xbb| + 2), p)] +  //  0 
+                        continuationClosure(xbb, p) +            //  1..|xbb|
+                    [(EVMProg2.Jump(-(|xbb| + 1)), p)]           //  |xbb| + 1
+                    +  toEVM(p[1..])
 
-            case IfElse(cond, xb1, xb2) => 
-                var xbb1 := toEVM(xb1);
-                var xbb2 := toEVM(xb2);
-                [EVMProg2.Jumpi(negF(cond), |xbb1| + 2)] +  // 0 
-                    xbb1 +                                  // 1..|xbb1|
-                [ EVMProg2.Jump(|xbb2| + 1)] +              //  |xbb1| + 1
-                    xbb2                                    //  |xbb1| + 2 to |xbb1| + 2 + |xbb2| - 1
+                case IfElse(cond, xb1, xb2) => 
+                    var xbb1 := toEVM(xb1);
+                    var xbb2 := toEVM(xb2);
+                    [(EVMProg2.Jumpi(negF(cond), |xbb1| + 2), xb2 + p[1..])] +  // 0 
+                        continuationClosure(xbb1, p[1..]) +                     // 1..|xbb1|
+                    [(EVMProg2.Jump(|xbb2| + 1), p[1..])] +                     //  |xbb1| + 1
+                        continuationClosure(xbb2, p[1..])                       //  |xbb1| + 2 to |xbb1| + 2 + |xbb2| - 1
+                    +  toEVM(p[1..])
     }
+
+    predicate equiv<S>(p:  seq<(EVMProg2, seq<EVMIRProg>)>, s1: (S, int), s2: (S, seq<EVMIRProg>))
+        // requires 0 <= s1.1 < |s1.2| 
+    {
+        &&  0 <= s1.1 < |p| 
+        &&  s1.0 == s2.0 
+        &&  p[s1.1].1 == s2.1 
+    }   
+
+    lemma simul<S>(p: seq<(EVMProg2, seq<EVMIRProg>)>, s1: (S, int), s2: (S, seq<EVMIRProg>))
+        // requires 0 <= s1.1 < |s1.2| 
+        requires equiv(p, s1, s2)
+        ensures 
+            var (pc1', s1') := stepEVM2(s1.1, p, s1.0);
+            var (s2', p2') := stepEVMIR(s2.1, s2.0);
+            equiv(p, (s1', pc1'), (s2', p2')) 
+    {
+        var (pc1', s1') := stepEVM2(s1.1, p, s1.0);
+        var (s2', p2') := stepEVMIR(s2.1, s2.0);
+        assume equiv(p, (s1', pc1'), (s2', p2')) ;
+    }
+
 
     /**
      *  Jumps in the translated EVMIR programs are within [0, |toEVM(p)|].
      *
      *  @param  p   An EVM-IR program.
      */
-    lemma {:verify false} toEVMIsClosed(p: EVMIRProg) 
-        ensures isClosed(toEVM(p))
-    {
-        match p 
-            case Block(i) => 
-            case While(c, Block(b)) => 
-            case IfElse(cond, Block(b1), Block(b2)) => 
-            case While(c, xb) => 
-                var xbb := toEVM(xb);
-                var whileEVM :=  
-                    [EVMProg2.Jumpi(negF(c), |xbb| + 2)] + 
-                        xbb + 
-                    [ EVMProg2.Jump(-(|xbb| + 1))];
-                assert toEVM(While(c, xb)) == whileEVM;
-                //  Prove closeness.
-                forall (i: nat | 0 <= i < |whileEVM|) 
-                    ensures closeJump(whileEVM, i)
-                {
-                    if 1 <= i < |whileEVM| - 1 {
-                        //  Instruction i in whileEVM is intruction i - 1 xbb 
-                        toEVMIsClosed(xb); 
-                        match whileEVM[i] 
-                            case Jumpi(cond, tgt) => 
-                                //  Jump must be to an instruction between 1 and |whileEVM| - 1
-                                calc ==> {
-                                    //  Induction on xbb
-                                    closeJump(xbb, i - 1);
-                                    0 <= i - 1 + tgt <= |xbb|;
-                                    calc == {
-                                        |xbb|;
-                                        |whileEVM| - 2;  
-                                    }
-                                    0 <= i - 1 + tgt <= |whileEVM| - 2;
-                                    1 <= i + tgt <= |whileEVM| - 1;
-                                    0 <= i + tgt <= |whileEVM|;
-                                }
-                            case Jump(tgt) => 
-                                //  Jump must be to an instruction between 1 and |whileEVM| - 1
-                                calc ==> {
-                                    closeJump(xbb, i - 1);
-                                    0 <= i - 1 + tgt <= |xbb|;
-                                    calc == {
-                                        |xbb|;
-                                        |whileEVM| - 2;   
-                                    }
-                                    0 <= i - 1 + tgt <= |whileEVM| - 2;
-                                    1 <= i + tgt <= |whileEVM| - 1;
-                                    0 <= i + tgt <= |whileEVM|;
-                                }
-                            case _ => 
-                    } else {
-                        //  i == 0 or i == |whileEVM| - 1
-                        assert closeJump(whileEVM, 0);
-                        assert closeJump(whileEVM, |whileEVM| - 1);
-                    }
-                }
-            case IfElse(cond, xb1, xb2) => 
-                var xbb1 := toEVM(xb1);
-                var xbb2 := toEVM(xb2);
-                var ifElseEVM := 
-                    [EVMProg2.Jumpi(negF(cond), |xbb1| + 2)] + //   0
-                        xbb1 +                      //  instructions from 1 to |xbb1|
-                    [EVMProg2.Jump(|xbb2| + 1)] +   //  instruction |xbb1| + 1
-                        xbb2;                       //  instructions from |xbb1| + 2 to |xbb1| + |xbb2| + 1
-                assert toEVM(IfElse(cond, xb1, xb2)) == ifElseEVM;
-                forall (i: nat | 0 <= i < |ifElseEVM|) 
-                    ensures closeJump(ifElseEVM, i)
-                {
-                    if 1 <= i <= |xbb1| {
-                        toEVMIsClosed(xb1);
-                        //  ifElseEVM[i] is xbb[i - 1]
-                        match ifElseEVM[i]
-                            case Jumpi(cond, tgt) => 
-                                 calc ==> {
-                                    closeJump(xbb1, i - 1);
-                                    0 <= i - 1 + tgt <= |xbb1|;
-                                    1 <= i + tgt <= |xbb1| + 1;
-                                    calc <= {
-                                        |xbb1| + 1;
-                                        |ifElseEVM|;  
-                                    }
-                                    0 <= i + tgt <= |ifElseEVM|; 
-                                }
-                            case Jump(tgt) => 
-                                calc ==> {
-                                    closeJump(xbb1, i - 1);
-                                    0 <= i - 1 + tgt <= |xbb1|;
-                                    1 <= i + tgt <= |xbb1| + 1;
-                                    calc <= {
-                                        |xbb1| + 1;
-                                        |ifElseEVM|;  
-                                    }
-                                    0 <= i + tgt <= |ifElseEVM|; 
-                                }
-                            case _ => 
-                    } else if |xbb1| + 2 <= i < |ifElseEVM| {
-                        toEVMIsClosed(xb2);
-                        //  ifElseEVM[i] is xbb2[i - (|xbb1| + 2)]
-                        match ifElseEVM[i]
-                            case Jumpi(cond, tgt) => 
-                                 calc ==> {
-                                    closeJump(xbb2, i - (|xbb1| + 2));
-                                    0 <= i - (|xbb1| + 2) + tgt <= |xbb2|;
-                                    |xbb1| + 2 <= i + tgt <=  |xbb2| + (|xbb1| + 2);
-                                    calc <= {
-                                        |xbb2| + (|xbb1| + 2);
-                                        |ifElseEVM|;  
-                                    }
-                                    0 <= i + tgt <= |ifElseEVM|; 
-                                }
-                            case Jump(tgt) => 
-                                calc ==> {
-                                    closeJump(xbb2, i - (|xbb1| + 2));
-                                    0 <= i - (|xbb1| + 2) + tgt <= |xbb2|;
-                                    |xbb1| + 2 <= i + tgt <=  |xbb2| + (|xbb1| + 2);
-                                    calc <= {
-                                        |xbb2| + (|xbb1| + 2);
-                                        |ifElseEVM|;  
-                                    }
-                                    0 <= i + tgt <= |ifElseEVM|; 
-                                }
-                            case _ => 
-                    } else {
-                        assert i == 0 || i == |xbb1| + 1;
-                        assert closeJump(ifElseEVM, i);
-                    } 
-                }
-    }
+    // lemma {:verify false} toEVMIsClosed(p: EVMIRProg) 
+    //     ensures isClosed(toEVM(p))
+    // {
+    //     match p 
+    //         case Block(i) => 
+    //         case While(c, Block(b)) => 
+    //         case IfElse(cond, Block(b1), Block(b2)) => 
+    //         case While(c, xb) => 
+    //             var xbb := toEVM(xb);
+    //             var whileEVM :=  
+    //                 [EVMProg2.Jumpi(negF(c), |xbb| + 2)] + 
+    //                     xbb + 
+    //                 [ EVMProg2.Jump(-(|xbb| + 1))];
+    //             assert toEVM(While(c, xb)) == whileEVM;
+    //             //  Prove closeness.
+    //             forall (i: nat | 0 <= i < |whileEVM|) 
+    //                 ensures closeJump(whileEVM, i)
+    //             {
+    //                 if 1 <= i < |whileEVM| - 1 {
+    //                     //  Instruction i in whileEVM is intruction i - 1 xbb 
+    //                     toEVMIsClosed(xb); 
+    //                     match whileEVM[i] 
+    //                         case Jumpi(cond, tgt) => 
+    //                             //  Jump must be to an instruction between 1 and |whileEVM| - 1
+    //                             calc ==> {
+    //                                 //  Induction on xbb
+    //                                 closeJump(xbb, i - 1);
+    //                                 0 <= i - 1 + tgt <= |xbb|;
+    //                                 calc == {
+    //                                     |xbb|;
+    //                                     |whileEVM| - 2;  
+    //                                 }
+    //                                 0 <= i - 1 + tgt <= |whileEVM| - 2;
+    //                                 1 <= i + tgt <= |whileEVM| - 1;
+    //                                 0 <= i + tgt <= |whileEVM|;
+    //                             }
+    //                         case Jump(tgt) => 
+    //                             //  Jump must be to an instruction between 1 and |whileEVM| - 1
+    //                             calc ==> {
+    //                                 closeJump(xbb, i - 1);
+    //                                 0 <= i - 1 + tgt <= |xbb|;
+    //                                 calc == {
+    //                                     |xbb|;
+    //                                     |whileEVM| - 2;   
+    //                                 }
+    //                                 0 <= i - 1 + tgt <= |whileEVM| - 2;
+    //                                 1 <= i + tgt <= |whileEVM| - 1;
+    //                                 0 <= i + tgt <= |whileEVM|;
+    //                             }
+    //                         case _ => 
+    //                 } else {
+    //                     //  i == 0 or i == |whileEVM| - 1
+    //                     assert closeJump(whileEVM, 0);
+    //                     assert closeJump(whileEVM, |whileEVM| - 1);
+    //                 }
+    //             }
+    //         case IfElse(cond, xb1, xb2) => 
+    //             var xbb1 := toEVM(xb1);
+    //             var xbb2 := toEVM(xb2);
+    //             var ifElseEVM := 
+    //                 [EVMProg2.Jumpi(negF(cond), |xbb1| + 2)] + //   0
+    //                     xbb1 +                      //  instructions from 1 to |xbb1|
+    //                 [EVMProg2.Jump(|xbb2| + 1)] +   //  instruction |xbb1| + 1
+    //                     xbb2;                       //  instructions from |xbb1| + 2 to |xbb1| + |xbb2| + 1
+    //             assert toEVM(IfElse(cond, xb1, xb2)) == ifElseEVM;
+    //             forall (i: nat | 0 <= i < |ifElseEVM|) 
+    //                 ensures closeJump(ifElseEVM, i)
+    //             {
+    //                 if 1 <= i <= |xbb1| {
+    //                     toEVMIsClosed(xb1);
+    //                     //  ifElseEVM[i] is xbb[i - 1]
+    //                     match ifElseEVM[i]
+    //                         case Jumpi(cond, tgt) => 
+    //                              calc ==> {
+    //                                 closeJump(xbb1, i - 1);
+    //                                 0 <= i - 1 + tgt <= |xbb1|;
+    //                                 1 <= i + tgt <= |xbb1| + 1;
+    //                                 calc <= {
+    //                                     |xbb1| + 1;
+    //                                     |ifElseEVM|;  
+    //                                 }
+    //                                 0 <= i + tgt <= |ifElseEVM|; 
+    //                             }
+    //                         case Jump(tgt) => 
+    //                             calc ==> {
+    //                                 closeJump(xbb1, i - 1);
+    //                                 0 <= i - 1 + tgt <= |xbb1|;
+    //                                 1 <= i + tgt <= |xbb1| + 1;
+    //                                 calc <= {
+    //                                     |xbb1| + 1;
+    //                                     |ifElseEVM|;  
+    //                                 }
+    //                                 0 <= i + tgt <= |ifElseEVM|; 
+    //                             }
+    //                         case _ => 
+    //                 } else if |xbb1| + 2 <= i < |ifElseEVM| {
+    //                     toEVMIsClosed(xb2);
+    //                     //  ifElseEVM[i] is xbb2[i - (|xbb1| + 2)]
+    //                     match ifElseEVM[i]
+    //                         case Jumpi(cond, tgt) => 
+    //                              calc ==> {
+    //                                 closeJump(xbb2, i - (|xbb1| + 2));
+    //                                 0 <= i - (|xbb1| + 2) + tgt <= |xbb2|;
+    //                                 |xbb1| + 2 <= i + tgt <=  |xbb2| + (|xbb1| + 2);
+    //                                 calc <= {
+    //                                     |xbb2| + (|xbb1| + 2);
+    //                                     |ifElseEVM|;  
+    //                                 }
+    //                                 0 <= i + tgt <= |ifElseEVM|; 
+    //                             }
+    //                         case Jump(tgt) => 
+    //                             calc ==> {
+    //                                 closeJump(xbb2, i - (|xbb1| + 2));
+    //                                 0 <= i - (|xbb1| + 2) + tgt <= |xbb2|;
+    //                                 |xbb1| + 2 <= i + tgt <=  |xbb2| + (|xbb1| + 2);
+    //                                 calc <= {
+    //                                     |xbb2| + (|xbb1| + 2);
+    //                                     |ifElseEVM|;  
+    //                                 }
+    //                                 0 <= i + tgt <= |ifElseEVM|; 
+    //                             }
+    //                         case _ => 
+    //                 } else {
+    //                     assert i == 0 || i == |xbb1| + 1;
+    //                     assert closeJump(ifElseEVM, i);
+    //                 } 
+    //             }
+    // }
 
     
 
@@ -199,136 +236,136 @@ module EVMIRSimulationFull {
      *
      *  @returns    The (minimum) number of steps in the EVMIR to simulate n steps in EVM. 
      */
-    lemma {:verify true} foo101<S>(xb: EVMIRProg, s: S, n: nat) returns (k: nat)
-        ensures isClosed(toEVM(xb))
-        ensures k <= n && runEVMIR3(xb, s, k).0 == runEVM3(0, toEVM(xb), s, n).0
-    {
-        toEVMIsClosed(xb);
-        if n < 1 {
-            k := 0;
-        } else {
-            match xb 
-                case Block(i) => 
-                    calc == {
-                        runEVM2(0, toEVM(xb), s, n).0;
-                        runEVM2(0, [EVMProg2.AInst(i)], s, n).0;
-                        runInst(i, s);
-                        runEVMIR3(Block(i), s, n).0;
-                        runEVMIR3(xb, s, n).0;
-                    }
-                    k := n ;
+    // lemma {:verify true} foo101<S>(xb: EVMIRProg, s: S, n: nat) returns (k: nat)
+    //     ensures isClosed(toEVM(xb))
+    //     ensures k <= n && runEVMIR3(xb, s, k).0 == runEVM3(0, toEVM(xb), s, n).0
+    // {
+    //     toEVMIsClosed(xb);
+    //     if n < 1 {
+    //         k := 0;
+    //     } else {
+    //         match xb 
+    //             case Block(i) => 
+    //                 calc == {
+    //                     runEVM2(0, toEVM(xb), s, n).0;
+    //                     runEVM2(0, [EVMProg2.AInst(i)], s, n).0;
+    //                     runInst(i, s);
+    //                     runEVMIR3(Block(i), s, n).0;
+    //                     runEVMIR3(xb, s, n).0;
+    //                 }
+    //                 k := n ;
 
-                case While(c, xb) => 
-                    var xbb := toEVM(xb);
-                    var whileEVM :=  [EVMProg2.Jumpi(negF(c), |xbb| + 2)] + xbb + [ EVMProg2.Jump(-(|xbb| + 2))];
-                    if c(s) {
-                        if n == 1 {
-                            k := n;
-                        } else {
-                            assert n >= 2;
-                            //  do one step in toEVM(While(c, xb))
-                            //  target state is s1 
-                            calc == {
-                                runEVM2(0, whileEVM, s, n);
-                                runEVM2(1, whileEVM, s, n - 1);
-                                // (s, |xbb| + 2);
-                            }  
-                            var (s', n') := runEVMIR2([xb], s, n - 1);
-                            //  From s1, run toEVM(xb). Match with k1 steps in xb
+    //             case While(c, xb) => 
+    //                 var xbb := toEVM(xb);
+    //                 var whileEVM :=  [EVMProg2.Jumpi(negF(c), |xbb| + 2)] + xbb + [ EVMProg2.Jump(-(|xbb| + 2))];
+    //                 if c(s) {
+    //                     if n == 1 {
+    //                         k := n;
+    //                     } else {
+    //                         assert n >= 2;
+    //                         //  do one step in toEVM(While(c, xb))
+    //                         //  target state is s1 
+    //                         calc == {
+    //                             runEVM2(0, whileEVM, s, n);
+    //                             runEVM2(1, whileEVM, s, n - 1);
+    //                             // (s, |xbb| + 2);
+    //                         }  
+    //                         var (s', n') := runEVMIR2([xb], s, n - 1);
+    //                         //  From s1, run toEVM(xb). Match with k1 steps in xb
 
-                            //  first n steps of toEVM(While(c, xb)) can be simulated by 
-                            //  1 + k1 
+    //                         //  first n steps of toEVM(While(c, xb)) can be simulated by 
+    //                         //  1 + k1 
 
-                            //  Then finish running
+    //                         //  Then finish running
 
-                            //  Use n - 1 steps to simulate toEVM(xb) 
-                            var (s1, n1) := runEVM2(0, toEVM(xb), s, n - 1);       
-                            if n1 < 2 {
-                                k := 0;
-                            } else {
-                                k := 1;
-                            }
-                            // calc == {
+    //                         //  Use n - 1 steps to simulate toEVM(xb) 
+    //                         var (s1, n1) := runEVM2(0, toEVM(xb), s, n - 1);       
+    //                         if n1 < 2 {
+    //                             k := 0;
+    //                         } else {
+    //                             k := 1;
+    //                         }
+    //                         // calc == {
 
-                            // }
-                            k := 0;
-                            assume runEVMIR3(While(c, xb), s, k).0 == runEVM3(0, toEVM(While(c, xb)), s, n).0;
-                        }
-                    } else {
-                        //  Condition is false, exit the loop and the jump program
-                        assert negF(c)(s);
-                        calc == {
-                            runEVM3(0, whileEVM, s, n).0;
-                            runEVM3(|xbb| + 1, whileEVM, s, n - 1).0;
-                            // (s, |xbb| + 1);
-                        }  
-                        //  In the while program, same state is reached in 1 step.
-                        calc == {
-                            runEVMIR3(While(c, xb), s, n);
-                            // runEVMIR3(, s , n - 1);
-                            (s, n - 1);
-                        }
-                        k := n;
-                    }
+    //                         // }
+    //                         k := 0;
+    //                         assume runEVMIR3(While(c, xb), s, k).0 == runEVM3(0, toEVM(While(c, xb)), s, n).0;
+    //                     }
+    //                 } else {
+    //                     //  Condition is false, exit the loop and the jump program
+    //                     assert negF(c)(s);
+    //                     calc == {
+    //                         runEVM3(0, whileEVM, s, n).0;
+    //                         runEVM3(|xbb| + 1, whileEVM, s, n - 1).0;
+    //                         // (s, |xbb| + 1);
+    //                     }  
+    //                     //  In the while program, same state is reached in 1 step.
+    //                     calc == {
+    //                         runEVMIR3(While(c, xb), s, n);
+    //                         // runEVMIR3(, s , n - 1);
+    //                         (s, n - 1);
+    //                     }
+    //                     k := n;
+    //                 }
 
-                case IfElse(c, xb1, xb2) => 
-                    var p := toEVM(IfElse(c, xb1, xb2));
-                        var xbb1 := toEVM(xb1);
-                        var xbb2 := toEVM(xb2);
-                        assert p == 
-                            [EVMProg2.Jumpi(negF(c), |xbb1| + 2)] +  // 0 
-                                xbb1 +                                  // 1..|xbb1|
-                            [ EVMProg2.Jump(|xbb2| + 1)] +              //  |xbb1| + 1
-                                xbb2;
-                    if c(s) {
-                        //  c(s) is true then execute xbb1
-                        // pcBoundsOnTermination(toEVM(xb1));
-                        //  Comopute new state and pc' and n'
-                        var (s', pc', n') := runEVM3(0, xbb1, s, n - 1);
+    //             case IfElse(c, xb1, xb2) => 
+    //                 var p := toEVM(IfElse(c, xb1, xb2));
+    //                     var xbb1 := toEVM(xb1);
+    //                     var xbb2 := toEVM(xb2);
+    //                     assert p == 
+    //                         [EVMProg2.Jumpi(negF(c), |xbb1| + 2)] +  // 0 
+    //                             xbb1 +                                  // 1..|xbb1|
+    //                         [ EVMProg2.Jump(|xbb2| + 1)] +              //  |xbb1| + 1
+    //                             xbb2;
+    //                 if c(s) {
+    //                     //  c(s) is true then execute xbb1
+    //                     // pcBoundsOnTermination(toEVM(xb1));
+    //                     //  Comopute new state and pc' and n'
+    //                     var (s', pc', n') := runEVM3(0, xbb1, s, n - 1);
 
-                        //  Get a simulation of xbb1 in k1 steps
-                        var k1 := foo101(xb1, s, n - 1);
-                        calc == {
-                            runEVM3(0, xbb1, s, n - 1).0;
-                            runEVMIR3(xb1, s, k1).0;
-                        }
-                        if pc' == |xbb1| {
-                            //  xbb1 could be run till the end 
+    //                     //  Get a simulation of xbb1 in k1 steps
+    //                     var k1 := foo101(xb1, s, n - 1);
+    //                     calc == {
+    //                         runEVM3(0, xbb1, s, n - 1).0;
+    //                         runEVMIR3(xb1, s, k1).0;
+    //                     }
+    //                     if pc' == |xbb1| {
+    //                         //  xbb1 could be run till the end 
 
-                        } else {
-                            //  xbb1 could not be run till the end
-                            //  p[1..|xbb1] is closed and actually equal to xbb1
-                            calc == {   //   to finish
-                                p[1..|xbb1|];
-                                ([EVMProg2.Jumpi(negF(c), |xbb1| + 2)] +  
-                                    xbb1 +                                
-                                [ EVMProg2.Jump(|xbb2| + 1)] +            
-                                    xbb2)[1..|xbb1|];  
-                            }
-                            assume p[1..|xbb1|] == xbb1;
-                            calc == {
-                                runEVM3(0, p, s, n);
-                                runEVM3(1, p, s, n - 1); 
-                                // runEVM2(0, xbb1, s, n - 1);
-                            }
+    //                     } else {
+    //                         //  xbb1 could not be run till the end
+    //                         //  p[1..|xbb1] is closed and actually equal to xbb1
+    //                         calc == {   //   to finish
+    //                             p[1..|xbb1|];
+    //                             ([EVMProg2.Jumpi(negF(c), |xbb1| + 2)] +  
+    //                                 xbb1 +                                
+    //                             [ EVMProg2.Jump(|xbb2| + 1)] +            
+    //                                 xbb2)[1..|xbb1|];  
+    //                         }
+    //                         assume p[1..|xbb1|] == xbb1;
+    //                         calc == {
+    //                             runEVM3(0, p, s, n);
+    //                             runEVM3(1, p, s, n - 1); 
+    //                             // runEVM2(0, xbb1, s, n - 1);
+    //                         }
                         
-                        // var (s', n') := runEVMIR2([xb1], s, n - 1);
-                        // calc == {
-                        //     runEVMIR2([IfElse(c, xb1, xb2)], s, n);
-                        //     runEVMIR2([], s', n - 1 - n');
-                        //     (s', n - 1 - n');
-                        }
-                        k := 1;
-                        assume runEVMIR3(IfElse(c, xb1, xb2), s, k).0 == runEVM3(0, toEVM(IfElse(c, xb1, xb2)), s, n).0;
+    //                     // var (s', n') := runEVMIR2([xb1], s, n - 1);
+    //                     // calc == {
+    //                     //     runEVMIR2([IfElse(c, xb1, xb2)], s, n);
+    //                     //     runEVMIR2([], s', n - 1 - n');
+    //                     //     (s', n - 1 - n');
+    //                     }
+    //                     k := 1;
+    //                     assume runEVMIR3(IfElse(c, xb1, xb2), s, k).0 == runEVM3(0, toEVM(IfElse(c, xb1, xb2)), s, n).0;
 
-                    } else {
-                        k := 1; 
-                        //  execute xb2 
-                        assume runEVMIR3(IfElse(c, xb1, xb2), s, k).0 == runEVM3(0, toEVM(IfElse(c, xb1, xb2)), s, n).0;
+    //                 } else {
+    //                     k := 1; 
+    //                     //  execute xb2 
+    //                     assume runEVMIR3(IfElse(c, xb1, xb2), s, k).0 == runEVM3(0, toEVM(IfElse(c, xb1, xb2)), s, n).0;
 
-                    }
-        }
-    }
+    //                 }
+    //     }
+    // }
         
     //  Translation proof (simple). Consistency check.
 
@@ -337,116 +374,116 @@ module EVMIRSimulationFull {
      *
      *  @returns    The (minimum) number of steps in the EVMIR to simulate n steps in EVM. 
      */
-    lemma {:verify false} singleWhileSim<S>(i: EVMInst, cond: S -> bool, n: nat, s: S) returns (k: nat)
-         ensures k <= n && runEVMIR([While(cond, Block(i))], s, k) ==
-            runEVM2(
-                0,
-                toEVM(While(cond, Block(i))),
-                s, 
-                n).0
-    {
-        //  For convenience and clarity, store program in a var 
-        var p :=  toEVM(While(cond, Block(i)));
-        if n < 2 {
-            //  Only one step can be simulated so the instruction at pc is not executed.
-            k := 0;
-        } else if n < 3 {
-            //  Exactly two steps in the EVM. 
-            assert n == 2;
-            if cond(s) {
-                k := 1;
-            } else {
-                assert !cond(s);
-                k := 0;
-            }
-        } else {
-            //  More than 2 steps in the EVM. So at least one iteration of the EVM body.
-            assert n > 2;
-            assert |toEVM(Block(i))| == 1;
-            if cond(s) {
-                calc == {
-                    runEVM2(0, p, s, n);
-                    runEVM2(1, p, s, n - 1);
-                    runEVM2(2, p, runInst(i, s), n - 2);
-                    runEVM2(0, p, runInst(i, s), n - 3);
-                }
-                //  Because body of while and jump progs are the same, they reach the same
-                //  state after one iteration of the body.
-                calc == {
-                    runEVMIR([While(cond, Block(i))], s, n);
-                    runEVMIR([While(cond, Block(i))], runInst(i, s), n - 1);
-                }
-                //  And by induction, we can get a simulation for the n - 3 remaining steps compute the same
-                //  result.
-                var xk := singleWhileSim(i, cond, n - 3, runInst(i, s));
-                //  Overall we do the body of the loop once and then in xk steps simulate the rest.
-                k := 1 + xk;
-            } else {
-                assert !cond(s);
-                //  Exit the loop.
-                k := 1;
-            }    
-        }
-    }    
+    // lemma {:verify false} singleWhileSim<S>(i: EVMInst, cond: S -> bool, n: nat, s: S) returns (k: nat)
+    //      ensures k <= n && runEVMIR([While(cond, Block(i))], s, k) ==
+    //         runEVM2(
+    //             0,
+    //             toEVM(While(cond, Block(i))),
+    //             s, 
+    //             n).0
+    // {
+    //     //  For convenience and clarity, store program in a var 
+    //     var p :=  toEVM(While(cond, Block(i)));
+    //     if n < 2 {
+    //         //  Only one step can be simulated so the instruction at pc is not executed.
+    //         k := 0;
+    //     } else if n < 3 {
+    //         //  Exactly two steps in the EVM. 
+    //         assert n == 2;
+    //         if cond(s) {
+    //             k := 1;
+    //         } else {
+    //             assert !cond(s);
+    //             k := 0;
+    //         }
+    //     } else {
+    //         //  More than 2 steps in the EVM. So at least one iteration of the EVM body.
+    //         assert n > 2;
+    //         assert |toEVM(Block(i))| == 1;
+    //         if cond(s) {
+    //             calc == {
+    //                 runEVM2(0, p, s, n);
+    //                 runEVM2(1, p, s, n - 1);
+    //                 runEVM2(2, p, runInst(i, s), n - 2);
+    //                 runEVM2(0, p, runInst(i, s), n - 3);
+    //             }
+    //             //  Because body of while and jump progs are the same, they reach the same
+    //             //  state after one iteration of the body.
+    //             calc == {
+    //                 runEVMIR([While(cond, Block(i))], s, n);
+    //                 runEVMIR([While(cond, Block(i))], runInst(i, s), n - 1);
+    //             }
+    //             //  And by induction, we can get a simulation for the n - 3 remaining steps compute the same
+    //             //  result.
+    //             var xk := singleWhileSim(i, cond, n - 3, runInst(i, s));
+    //             //  Overall we do the body of the loop once and then in xk steps simulate the rest.
+    //             k := 1 + xk;
+    //         } else {
+    //             assert !cond(s);
+    //             //  Exit the loop.
+    //             k := 1;
+    //         }    
+    //     }
+    // }    
         
     /**
      *  If Then Else Simulation proof. Assume unique block in ifBody and ifElse.
      *
      *  @returns    The (minimum) number of steps in the EVMIR to simulate n steps in EVM. 
      */
-    lemma {:verify false} ifTheElseSim<S>(i1: EVMInst, i2: EVMInst, cond: S -> bool, n: nat, s: S) returns (k: nat)
-        requires n > 2
-        ensures k <= n && runEVMIR([IfElse(cond, Block(i1), Block(i2))], s, k) ==  
-            runEVM2(
-                0,
-                toEVM(IfElse(cond, Block(i1), Block(i2))),
-                s, 
-                n).0
-    { 
-        var p := toEVM(IfElse(cond, Block(i1), Block(i2)));
-        if n < 3 {
-            //  if less than 1 step, only evaluate condition which takes no steps in EVM-IR
-            if n <= 1 {
-                k := 0 ;
-            } else {
-                //  Evaluate condition and execute i1 or i2. One step in EVM-IR
-                k := 1;
-            }
-        } else {
-            assert |toEVM(Block(i1))| == 1;
-            assert |toEVM(Block(i2))| == 1; 
-            if cond(s) {
-                //  Execute the ifBody
-                calc == {
-                    runEVM2(0, p, s, n);
-                    runEVM2(1, p, s, n - 1);
-                    runEVM2(2, p, runInst(i1, s), n - 2);
-                    runEVM2(4, p, runInst(i1, s), n - 3);
-                }
-                //  EVM-IR program simulates p in 2 steps
-                calc == {
-                    runEVMIR([IfElse(cond, Block(i1), Block(i2))], s, n);
-                    runEVMIR([], runInst(i1, s), n - 1);
-                    runInst(i1, s);
-                }
-                k := n - 2;
-            } else {
-                assert !cond(s);
-                calc == {
-                    runEVM2(0, p, s, n);
-                    runEVM2(3, p, s, n - 1);
-                    runEVM2(4, p, runInst(i2, s), n - 2);
-                }
-                //  EVM-IR program simulates p in 2 steps
-                calc == {
-                    runEVMIR([IfElse(cond, Block(i1), Block(i2))], s, n);
-                    runEVMIR([], runInst(i2, s), n - 1);
-                    runInst(i2, s);
-                }
-                k := n - 2;
-            }
-        }
-    }
+    // lemma {:verify false} ifTheElseSim<S>(i1: EVMInst, i2: EVMInst, cond: S -> bool, n: nat, s: S) returns (k: nat)
+    //     requires n > 2
+    //     ensures k <= n && runEVMIR([IfElse(cond, Block(i1), Block(i2))], s, k) ==  
+    //         runEVM2(
+    //             0,
+    //             toEVM(IfElse(cond, Block(i1), Block(i2))),
+    //             s, 
+    //             n).0
+    // { 
+    //     var p := toEVM(IfElse(cond, Block(i1), Block(i2)));
+    //     if n < 3 {
+    //         //  if less than 1 step, only evaluate condition which takes no steps in EVM-IR
+    //         if n <= 1 {
+    //             k := 0 ;
+    //         } else {
+    //             //  Evaluate condition and execute i1 or i2. One step in EVM-IR
+    //             k := 1;
+    //         }
+    //     } else {
+    //         assert |toEVM(Block(i1))| == 1;
+    //         assert |toEVM(Block(i2))| == 1; 
+    //         if cond(s) {
+    //             //  Execute the ifBody
+    //             calc == {
+    //                 runEVM2(0, p, s, n);
+    //                 runEVM2(1, p, s, n - 1);
+    //                 runEVM2(2, p, runInst(i1, s), n - 2);
+    //                 runEVM2(4, p, runInst(i1, s), n - 3);
+    //             }
+    //             //  EVM-IR program simulates p in 2 steps
+    //             calc == {
+    //                 runEVMIR([IfElse(cond, Block(i1), Block(i2))], s, n);
+    //                 runEVMIR([], runInst(i1, s), n - 1);
+    //                 runInst(i1, s);
+    //             }
+    //             k := n - 2;
+    //         } else {
+    //             assert !cond(s);
+    //             calc == {
+    //                 runEVM2(0, p, s, n);
+    //                 runEVM2(3, p, s, n - 1);
+    //                 runEVM2(4, p, runInst(i2, s), n - 2);
+    //             }
+    //             //  EVM-IR program simulates p in 2 steps
+    //             calc == {
+    //                 runEVMIR([IfElse(cond, Block(i1), Block(i2))], s, n);
+    //                 runEVMIR([], runInst(i2, s), n - 1);
+    //                 runInst(i2, s);
+    //             }
+    //             k := n - 2;
+    //         }
+    //     }
+    // }
 
 
 }
