src/dafny/refinement/evmir.dfy
@@ -25,8 +25,42 @@ module EVMIR {
     /** Programs with block of instructions, while loops/ifs. */
     datatype EVMIRProg<!S> =  
         |   Block(i:EVMInst)
-        |   While(cond: S -> bool, body: EVMIRProg)
-        |   IfElse(cond: S -> bool, ifBody: EVMIRProg, elseBody: EVMIRProg) 
+        // |   Sequence(p1: EVMIRProg, p2: EVMIRProg)
+        |   While(cond: S -> bool, body: seq<EVMIRProg>)
+        |   IfElse(cond: S -> bool, ifBody: seq<EVMIRProg>, elseBody: seq<EVMIRProg>) 
+        // |   Skip()
+
+    /**
+     *  Semantics of EVMIR programs.
+     *
+     *  @param  p   An EVMIR program.
+     *  @param  s   A state.
+     *  @returns    The state obtained after executing one step of `p` from `s`,
+     *              and the program that is left to be executed.
+     */
+    function method stepEVMIR<S>(p: seq<EVMIRProg>, s: S): (S, seq<EVMIRProg>) 
+    {   
+        if |p| == 0 then (s, [])
+        else 
+            match p[0]
+                case Block(i) => (runInst(i, s), p[1..])
+                // case Sequence(b1, b2) => 
+                //     var (s', p') := stepEVMIR(b1, s);
+                //     (s', Sequence(p', p))
+                case While(c, b) => 
+                        if c(s) then
+                            var (s', p') := stepEVMIR(b, s);
+                            (s', p' + p)
+                        else 
+                            (s, p[1..])
+                case IfElse(c, b1, b2) => 
+                    if c(s) then 
+                        var (s', p') := stepEVMIR(b1, s);
+                        (s', p' + p[1..])
+                    else var (s', p') := stepEVMIR(b2, s);
+                        (s', p' + p[1..])
+                // case Skip() => (s, Skip)
+    }
 
     /**
      *  Run n steps of the program.
@@ -37,23 +71,23 @@ module EVMIR {
      *  @param  n   The number of steps to execute.
      *  @returns    The state obtained after executing `n` steps of `p`. 
      */
-    function method runEVMIR<S>(p: seq<EVMIRProg>, s: S, n: nat): S 
-        decreases n - 1
-    {   
-        if n == 0 || p == [] then s 
-            //  max number of steps reached or program has terminated. 
-        else 
-            match p[0] 
-                case Block(i) => runInst(i, s)
-                case While(c, Block(b)) => 
-                    if c(s) then runEVMIR(p, runInst(b, s), n - 1)
-                    else runEVMIR(p[1..], s , n - 1)
-                case While(c, b) => s   // Todo
-                case IfElse(c, Block(b1), Block(b2)) => 
-                    if c(s) then runEVMIR(p[1..], runInst(b1, s), n - 1)
-                    else  runEVMIR(p[1..], runInst(b2, s), n - 1)
-                 case IfElse(c, _, _) =>  s   // Todo
-    }
+    // function method runEVMIR<S>(p: seq<EVMIRProg>, s: S, n: nat): S 
+    //     decreases n - 1
+    // {   
+    //     if n == 0 || p == [] then s 
+    //         //  max number of steps reached or program has terminated. 
+    //     else 
+    //         match p[0] 
+    //             case Block(i) => runInst(i, s)
+    //             case While(c, Block(b)) => 
+    //                 if c(s) then runEVMIR(p, runInst(b, s), n - 1)
+    //                 else runEVMIR(p[1..], s , n - 1)
+    //             case While(c, b) => s   // Todo
+    //             case IfElse(c, Block(b1), Block(b2)) => 
+    //                 if c(s) then runEVMIR(p[1..], runInst(b1, s), n - 1)
+    //                 else  runEVMIR(p[1..], runInst(b2, s), n - 1)
+    //              case IfElse(c, _, _) =>  s   // Todo
+    // }
 
     /**
      *  Interpretation of EVM-IR.
@@ -66,42 +100,42 @@ module EVMIR {
      *
      *  @note       In this interpretation a test for a condition costs 1.
      */
-    function method runEVMIR2<S>(p: seq<EVMIRProg>, s: S, n: nat): (S, nat) 
-        ensures runEVMIR2(p, s, n).1 <= n 
-        ensures n > 0 && p != [] ==> runEVMIR2(p, s, n).1 < n
-        decreases n - 1
-    {   
-        if n == 0 || p == [] then (s, n) 
-            //  max number of steps reached or program has terminated. 
-        else 
-            match p[0] 
-                case Block(i) => (runInst(i, s), n - 1)
-                case While(c, b) => 
-                    if c(s) then 
-                        var (s', n') := runEVMIR2([b], s, n - 1);
-                        runEVMIR2(p, s', n - 1 - n')
-                    else runEVMIR2(p[1..], s , n - 1)
-                case IfElse(c, b1, b2) => 
-                    var (s', n') := if c(s) then runEVMIR2([b1], s, n - 1) else runEVMIR2([b2], s, n - 1);
-                    runEVMIR2(p[1..], s', n - 1 - n')
-    }
+    // function method runEVMIR2<S>(p: seq<EVMIRProg>, s: S, n: nat): (S, nat) 
+    //     ensures runEVMIR2(p, s, n).1 <= n 
+    //     ensures n > 0 && p != [] ==> runEVMIR2(p, s, n).1 < n
+    //     decreases n - 1
+    // {   
+    //     if n == 0 || p == [] then (s, n) 
+    //         //  max number of steps reached or program has terminated. 
+    //     else 
+    //         match p[0] 
+    //             case Block(i) => (runInst(i, s), n - 1)
+    //             case While(c, b) => 
+    //                 if c(s) then 
+    //                     var (s', n') := runEVMIR2([b], s, n - 1);
+    //                     runEVMIR2(p, s', n - 1 - n')
+    //                 else runEVMIR2(p[1..], s , n - 1)
+    //             case IfElse(c, b1, b2) => 
+    //                 var (s', n') := if c(s) then runEVMIR2([b1], s, n - 1) else runEVMIR2([b2], s, n - 1);
+    //                 runEVMIR2(p[1..], s', n - 1 - n')
+    // }
 
-    function method runEVMIR3<S>(p: EVMIRProg, s: S, n: nat): (S, nat) 
-        ensures runEVMIR3(p, s, n).1 <= n 
-        // ensures n > 0 && p != [] ==> runEVMIR2(p, s, n).1 < n
-        decreases n - 1
-    {   
-        if n == 0 then (s, n) 
-            //  max number of steps reached or program has terminated. 
-        else 
-            match p
-                case Block(i) => (runInst(i, s), n - 1)
-                case While(c, b) => 
-                    if c(s) then 
-                        var (s', n') := runEVMIR3(b, s, n - 1);
-                        runEVMIR3(p, s', n - 1 - n')
-                    else (s , n - 1)
-                case IfElse(c, b1, b2) => 
-                    if c(s) then runEVMIR3(b1, s, n - 1) else runEVMIR3(b2, s, n - 1)
-    }
+    // function method runEVMIR3<S>(p: EVMIRProg, s: S, n: nat): (S, nat) 
+    //     ensures runEVMIR3(p, s, n).1 <= n 
+    //     // ensures n > 0 && p != [] ==> runEVMIR2(p, s, n).1 < n
+    //     decreases n - 1
+    // {   
+    //     if n == 0 then (s, n) 
+    //         //  max number of steps reached or program has terminated. 
+    //     else 
+    //         match p
+    //             case Block(i) => (runInst(i, s), n - 1)
+    //             case While(c, b) => 
+    //                 if c(s) then 
+    //                     var (s', n') := runEVMIR3(b, s, n - 1);
+    //                     runEVMIR3(p, s', n - 1 - n')
+    //                 else (s , n - 1)
+    //             case IfElse(c, b1, b2) => 
+    //                 if c(s) then runEVMIR3(b1, s, n - 1) else runEVMIR3(b2, s, n - 1)
+    // }
 }
